done with revising 2.4 under the new definitions

chap2_4revisedScript.sml
@@ -50,6 +50,21 @@ val fAND_def = Define`
   fAND ff1 ff2 = fNOT (fDISJ (fNOT ff1) (fNOT ff2))`;
 
 
+val tvars_def = Define`
+  tvars (fVar a) = {a} /\
+  tvars (fConst a) = {}`;
+
+val fvars_def = Define`
+  fvars (fRrel a t1 t2) = tvars t1 ∪ tvars t2 /\
+  fvars (fPrel a t) = tvars t /\
+  fvars (fDISJ ff1 ff2) = (fvars ff1) ∪ (fvars ff2) /\
+  fvars (fNOT ff) = fvars ff /\
+  fvars (fEXISTS n ff) = n INSERT (fvars ff) /\
+  fvars (fEQ t1 t2) = tvars t1 ∪ tvars t2`;
+
+
+
+
 val ST_def = Define`
   (ST x (u:unit) (VAR p) <=> fPrel p (fVar x)) /\
   (ST x u (FALSE) <=> fNOT (fEQ (fVar x) (fVar x))) /\
@@ -122,19 +137,168 @@ val prop_2_47_i = store_thm(
 
 
 
+val fFORALL_def = Define`
+  fFORALL n ff = fNOT (fEXISTS n (fNOT ff))`;
 
 
-val tvars_def = Define`
-  tvars (fVar a) = {a} /\
-  tvars (fConst a) = {}`;
+val prop_2_47_ii = store_thm(
+  "prop_2_47_ii",
+  ``!phi M. universal_true M phi <=> (!σ. IMAGE σ univ(:num) SUBSET M.frame.world ==> (fsatis (mm2folm M) σ (fFORALL x (ST x u phi))))``,
+  rw[universal_true_def,fFORALL_def,fsatis_def,feval_def] >> rw[EQ_IMP_THM] (* 3 *)
+  >- fs[mm2folm_def]
+  >- (`!x'. x' IN (mm2folm M).domain ==> feval (mm2folm M) ((x =+ x') σ) (ST x () phi)` suffices_by metis_tac[] >> rw[] >>
+     `fsatis (mm2folm M) ((x =+ x') σ) (ST x () phi)` suffices_by metis_tac[fsatis_def] >>
+     `x' IN M.frame.world` by fs[mm2folm_def] >>
+     `satis M x' phi` by metis_tac[] >>
+     `IMAGE ((x =+ x') σ) 𝕌(:num) ⊆ M.frame.world`
+         by (rw[IMAGE_DEF,SUBSET_DEF] >> Cases_on `x''' = x` >> rw[APPLY_UPDATE_THM] >> fs[SUBSET_DEF,IMAGE_DEF] >> metis_tac[]) >>
+     `((x =+ x') σ) x = x'` by fs[APPLY_UPDATE_THM] >> metis_tac[prop_2_47_i])
+  >- (`IMAGE (\n.w) 𝕌(:num) ⊆ M.frame.world`
+         by (rw[IMAGE_DEF,SUBSET_DEF] >> metis_tac[]) >>
+     `∀x'.
+            x' IN (mm2folm M).domain ==>
+            feval (mm2folm M) ((x =+ x') (\n.w)) (ST x () phi)` by metis_tac[] >>
+     `w IN (mm2folm M).domain` by fs[mm2folm_def] >>
+     `feval (mm2folm M) ((x =+ w) (λn. w)) (ST x () phi)` by metis_tac[] >>
+     `IMAGE ((x =+ w) (λn. w)) 𝕌(:num) ⊆ M.frame.world`
+         by (rw[IMAGE_DEF,SUBSET_DEF] >> Cases_on `x'' = x` >> rw[APPLY_UPDATE_THM]) >>
+     `fsatis (mm2folm M) ((x =+ w) (λn. w)) (ST x () phi)` by metis_tac[fsatis_def] >>
+     `((x =+ w) (λn. w)) x = w` by fs[APPLY_UPDATE_THM] >>
+     imp_res_tac prop_2_47_i >> metis_tac[]));
+     
+  
 
-val fvars_def = Define`
-  fvars (fRrel a t1 t2) = tvars t1 ∪ tvars t2 /\
-  fvars (fPrel a t) = tvars t /\
-  fvars (fDISJ ff1 ff2) = (fvars ff1) ∪ (fvars ff2) /\
-  fvars (fNOT ff) = fvars ff /\
-  fvars (fEXISTS n ff) = n INSERT (fvars ff) /\
-  fvars (fEQ t1 t2) = tvars t1 ∪ tvars t2`;
+
+val ST_alt_def = Define`
+  (ST_alt x u (VAR p) <=> fPrel p (fVar x)) /\
+  (ST_alt x u (FALSE) <=> fNOT (fEQ (fVar x) (fVar x))) /\
+  (ST_alt x u (NOT phi) <=> fNOT (ST_alt x u phi)) /\
+  (ST_alt x u (DISJ phi psi) <=> fDISJ (ST_alt x u phi) (ST_alt x u psi)) /\
+  (ST_alt x u (DIAM phi) <=> fEXISTS (1 - x) (fAND (fRrel u (fVar x) (fVar (1 - x))) (ST_alt (1 - x) u phi)))`;
+
+
+val prop_2_47_i_alt = store_thm(
+  "prop_2_47_i_alt",
+  ``!M w:'b phi σ. (IMAGE σ univ(:num)) SUBSET M.frame.world
+                       ==> (satis M (σ 1) phi <=> fsatis (mm2folm M) σ (ST_alt 1 u phi)) /\
+		           (satis M (σ 0) phi <=> fsatis (mm2folm M) σ (ST_alt 0 u phi))``,
+  Induct_on `phi` >> rw[] (* 10 *)
+  >- (rw[feval_def,ST_alt_def,fsatis_def] >> eq_tac >> rw[] (* 3 *)
+     >- rw[mm2folm_def]
+     >- (rw[mm2folm_def,interpret_def] (* 2 *)
+        >> metis_tac[satis_def,IN_DEF])
+     >- (fs[mm2folm_def,interpret_def] >> rw[satis_def] >> metis_tac[IN_DEF]))
+  >- (rw[feval_def,ST_alt_def,fsatis_def,mm2folm_def,interpret_def] >> eq_tac >> rw[] (* 3 *)
+     >- metis_tac[satis_def,IN_DEF]
+     >- metis_tac[satis_def,IN_DEF]
+     >- (rw[satis_def] >> metis_tac[IN_DEF]))
+  >- (fs[satis_def,feval_def,ST_alt_def,fsatis_def,mm2folm_def,interpret_def])
+  >- (fs[satis_def,feval_def,ST_alt_def,fsatis_def,mm2folm_def,interpret_def])
+  >- (fs[satis_def,feval_def,ST_alt_def,fsatis_def,mm2folm_def,interpret_def])
+  >- (fs[satis_def,feval_def,ST_alt_def,fsatis_def,mm2folm_def,interpret_def])
+  >- (rw[satis_def,feval_def,ST_alt_def,fsatis_def] >> eq_tac >> rw[] (* 5 *)
+     >- fs[mm2folm_def]
+     >- fs[mm2folm_def]
+     >- fs[mm2folm_def]
+     >- fs[]
+     >- (fs[IMAGE_DEF,SUBSET_DEF] >> metis_tac[]))
+  >- (rw[satis_def,feval_def,ST_alt_def,fsatis_def] >> eq_tac >> rw[] (* 5 *)
+     >- fs[mm2folm_def]
+     >- fs[mm2folm_def]
+     >- fs[mm2folm_def]
+     >- fs[mm2folm_def]
+     >- (fs[IMAGE_DEF,SUBSET_DEF] >> metis_tac[]))
+  >- (rw[satis_def,feval_def,ST_alt_def,fsatis_def] >> eq_tac >> rw[] (* 4 *)
+     >- fs[mm2folm_def]
+     >- (qexists_tac `v` >> rw[fAND_def,feval_def,APPLY_UPDATE_THM] (* 3 *)
+        >- fs[mm2folm_def]
+	>- rw[mm2folm_def,interpret_def,APPLY_UPDATE_THM] 
+	>- (fs[fsatis_def] >>
+           `((0 =+ v) σ) 0 = v` by rw[APPLY_UPDATE_THM] >>
+           `IMAGE ((0 =+ v) σ) 𝕌(:num) ⊆ M.frame.world`
+	       by (rw[IMAGE_DEF,SUBSET_DEF] >> Cases_on `x' = 0` (* 2 *)
+	           >> rw[APPLY_UPDATE_THM] >> fs[IMAGE_DEF,SUBSET_DEF] >> metis_tac[]) >>
+	   metis_tac[]))
+     >- (fs[SUBSET_DEF,IMAGE_DEF] >> metis_tac[])
+     >- (qexists_tac `x` >> rw[] (* 3 *)
+        >- fs[feval_def,fAND_def,fsatis_def,mm2folm_def,interpret_def,APPLY_UPDATE_THM]
+        >- fs[mm2folm_def]
+	>- (fs[feval_def,fAND_def,fsatis_def] >>
+	   `IMAGE ((0 =+ x) σ) 𝕌(:num) ⊆ M.frame.world`
+	   by (rw[IMAGE_DEF,SUBSET_DEF] >> Cases_on `x'' = 0` (* 2 *)
+	      >> rw[APPLY_UPDATE_THM] >> fs[IMAGE_DEF,SUBSET_DEF,mm2folm_def] >> metis_tac[]) >>
+	   `((0 =+ x) σ) 0 = x` by fs[APPLY_UPDATE_THM] >>
+	   `IMAGE ((0 =+ x) σ) 𝕌(:num) ⊆ (mm2folm M).domain` by fs[mm2folm_def] >>
+	   metis_tac[mm2folm_def])))
+  >- (rw[satis_def,feval_def,ST_alt_def,fsatis_def] >> eq_tac >> rw[] (* 4 *)
+     >- fs[mm2folm_def]
+     >- (qexists_tac `v` >> rw[fAND_def,feval_def,APPLY_UPDATE_THM] (* 3 *)
+        >- fs[mm2folm_def]
+	>- rw[mm2folm_def,interpret_def,APPLY_UPDATE_THM] 
+        >- (fs[fsatis_def] >>
+           `((1 =+ v) σ) 1= v` by rw[APPLY_UPDATE_THM] >>
+           `IMAGE ((1 =+ v) σ) 𝕌(:num) ⊆ M.frame.world`
+	       by (rw[IMAGE_DEF,SUBSET_DEF] >> Cases_on `x' = 1` (* 2 *)
+	          >> rw[APPLY_UPDATE_THM] >> fs[IMAGE_DEF,SUBSET_DEF] >> metis_tac[]) >>
+           metis_tac[]))
+     >- (fs[SUBSET_DEF,IMAGE_DEF] >> metis_tac[])
+     >- (qexists_tac `x` >> rw[] (* 3 *)
+        >- fs[feval_def,fAND_def,fsatis_def,mm2folm_def,interpret_def,APPLY_UPDATE_THM]
+        >- fs[mm2folm_def]
+        >- (fs[feval_def,fAND_def,fsatis_def] >>
+	   `IMAGE ((1 =+ x) σ) 𝕌(:num) ⊆ M.frame.world`
+	   by (rw[IMAGE_DEF,SUBSET_DEF] >> Cases_on `x'' = 0` (* 2 *)
+	      >> rw[APPLY_UPDATE_THM] >> fs[IMAGE_DEF,SUBSET_DEF,mm2folm_def] >> metis_tac[]) >>
+	   `((1 =+ x) σ) 1 = x` by fs[APPLY_UPDATE_THM] >>
+	   `IMAGE ((1 =+ x) σ) 𝕌(:num) ⊆ (mm2folm M).domain` by fs[mm2folm_def] >>
+	   metis_tac[mm2folm_def]))));
+
+
+val ST_alt_two_var = store_thm(
+  "ST_alt_two_var",
+  ``!phi. fvars (ST_alt 0 u phi) SUBSET {0;1} /\ fvars (ST_alt 1 u phi) SUBSET {0;1}``,
+  Induct_on `phi` >> rw[] >> fs[ST_alt_def,fvars_def,SUBSET_DEF,tvars_def] >> rw[]
+  >- metis_tac[]
+  >- metis_tac[]
+  >- metis_tac[]
+  >- metis_tac[]
+  >> fs[fAND_def,fvars_def,tvars_def]);
+
+
+
+
+
+
+val fequiv_def = Define`
+  fequiv (μ:'b itself) ff1 ff2 <=> (!M (σ:num -> 'b). (IMAGE σ univ(:num)) SUBSET M.frame.world
+                                                        ==> (fsatis (mm2folm M) σ ff1 <=> fsatis (mm2folm M) σ ff2))`;
+
+
+
+val ST_ST_alt_fequiv = store_thm(
+  "ST_ST_alt_fequiv",
+  ``!phi. fequiv μ (ST 0 u phi) (ST_alt 0 u phi) /\ fequiv μ (ST 1 u phi) (ST_alt 1 u phi)``,
+  rw[ST_alt_def,ST_def,fequiv_def] (* 2 *)
+  >- (eq_tac >> rw[] (* 2 *)
+     >- (`satis M (σ 0) phi` by metis_tac[prop_2_47_i] >>
+        metis_tac[prop_2_47_i_alt])
+     >- metis_tac[prop_2_47_i_alt,prop_2_47_i])
+  >- metis_tac[prop_2_47_i,prop_2_47_i_alt]);
+
+
+
+
+  
+val prop_2_49_i = store_thm(
+  "prop_2_49_i",
+  ``!phi. ?fphi. (fvars fphi) SUBSET {0;1} /\
+                 fequiv μ (ST 0 u phi) fphi``,
+  rw[] >> qexists_tac `(ST_alt 0 u phi)` >>
+  `u = ()` by fs[] >>
+  metis_tac[ST_alt_two_var,ST_ST_alt_fequiv]);
+
+
+
 
 
 val tconsts_def = Define`
@@ -410,7 +574,17 @@ val thm_2_65 = store_thm(
 	     
 		  
 		  
-	       
+val invariant_for_bisim_def = Define`
+  invariant_for_bisim (a:'a itself) (b:'b itself) ff x <=> freevars ff SUBSET {x} /\
+                               !M N w v. bisim_world M N (w:'a) (v:'b) ==>
+			       (!σ1 σ2.
+			        IMAGE σ1 univ(:num) SUBSET M.frame.world /\
+				IMAGE σ2 univ(:num) SUBSET N.frame.world ==>
+                                (fsatis (mm2folm M) ((x =+ w)σ1) ff <=> fsatis (mm2folm N) ((x =+ v)σ2) ff))`;
+
+val thm_2_68 = store_thm(
+  "thm_2_68",
+  ``
 	          
 	    
 	 
